Frame rule is Back

theories/Logic/Sim.v
@@ -7,62 +7,85 @@ From RSL.Simulations Require Export FreeSim.
 
 From RSL.Logic Require Import rPropDef Tactic.
 
-Program Definition sim_lfp {Λt Λs J I} Pt Ps C st j i ss Q : rProp :=
+Program Definition sim_def {Λt Λs J I} Pt Ps C t j i s Q : rProp :=
   {|
     rProp_holds mt ms :=
       let Ψ vt vs := rProp_holds (Q vt vs : rProp)
-      in elem (C: Chain (@fsim_lfp Λt Λs J I Pt Ps)) Ψ (st, mt) j i (ss, ms)
+      in elem (C: Chain (@fsim_lfp Λt Λs J I Pt Ps)) Ψ (t, mt) j i (s, ms)
   |}.
 
+Definition sim {Λt Λs J I} Pt Ps C t j i s Q : rProp :=
+  ∀ P, P -∗ @sim_def Λt Λs J I Pt Ps C t j i s (fun vt vs => Q vt vs ∗ P).
+
 Notation
-  "'[' Pt ',' Ps ',' C ']' st '<{' j ',' i '}=' ss '{{' Q '}}'" :=
-  (sim_lfp Pt Ps C st j i ss Q%I)
-    (at level 0, st at level 0, ss at level 0, no associativity).
+  "'[' Pt ',' Ps ',' C ']' t '<{' j ',' i '}=' s '{{' Q '}}'" :=
+  (sim Pt Ps C t j i s Q%I)
+    (at level 0, t at level 0, s at level 0, no associativity).
 
 Section SimRules.
   Context {Λt Λs: lang} {J I: WfRel}.
   Context {Pt: prog Λt} {Ps: prog Λs}.
   Context {C: Chain (fsim_lfp J I Pt Ps)}.
 
-  Implicit Types (st: state Λt) (j: J) (i: I) (ss: state Λs)
+  Implicit Types (t: state Λt) (j: J) (i: I) (s: state Λs)
     (Q: value Λt -> value Λs -> rProp).
 
-  Lemma final st j i ss Q vt vs:
-    is_value st = Some vt ->
-    is_value ss = Some vs ->
+  Lemma final t j i s Q vt vs:
+    is_value t = Some vt ->
+    is_value s = Some vs ->
     Q vt vs -∗
-    [Pt, Ps, C] st <{j, i}= ss {{ Q }}.
+    [Pt, Ps, C] t <{j, i}= s {{ Q }}.
   Proof using Type.
     intros Ht Hs.
-    unseal. intros ? ? [-> ->] mt ms _ _ Hp. smap.
+    unfold sim. unseal.
+    intros ? ? [-> ->] mtQ msQ _ _ Hq. smap.
+    intros W mtW msW Hdt Hds HW. simpl.
     apply chain_related.
-    eexists _, _, _, _. split_and!.
-    - simpl. by rewrite Ht.
-    - simpl. by rewrite Hs.
-    - simpl. assumption.
+    eexists _, _, _, _. split_and!; simpl.
+    - by rewrite Ht.
+    - by rewrite Hs.
+    - exists mtQ, msQ, mtW, msW. by split_and!.
   Qed.
 
   Lemma sim_mono st j i ss Q j' i' Q':
-    □ (∀ vt vs, Q' vt vs -∗ Q vt vs) -∗
+    (∀ vt vs, Q' vt vs -∗ Q vt vs) -∗
     ⌜j ⊑ j'⌟ -∗
     ⌜i ⊑ i'⌟ -∗
     [Pt, Ps, C] st <{j, i}= ss {{ Q' }} -∗
     [Pt, Ps, C] st <{j', i'}= ss {{ Q }}.
   Proof using Type.
-    unseal.
+    unfold sim. unseal.
     intros ? ? [-> ->].
-    intros mtP msP _ _ [[-> ->] HQ].
+    intros mtQ msQ _ _ HQ.
     intros ? ? _ _ [[-> ->] Hj].
     intros ? ? _ _ [[-> ->] Hi].
-    intros mt ms _ _ Hsim. smap.
-    simpl in *.
-    eapply chain_mono; last done.
-    - intros vt vs mt' ms' H.
-      replace (mt') with (∅ ∪ mt') by smap.
-      replace (ms') with (∅ ∪ ms') by smap.
-      apply HQ.
-      + by apply map_disjoint_empty_r.
-      + by apply map_disjoint_empty_r.
+    intros mt ms ? ? Hsim.
+    intros W mtW msW ? ? HW. smap.
+    simpl in *. decompose_map_disjoint.
+    eapply chain_mono.
+    4:{
+      replace (mtQ ∪ mt ∪ mtW) with (mt ∪ (mtQ ∪ mtW)).
+      2:{ smap. f_equal. by apply map_union_comm. }
+      replace (msQ ∪ ms ∪ msW) with (ms ∪ (msQ ∪ msW)).
+      2:{ smap. f_equal. by apply map_union_comm. }
+      apply Hsim.
+      - solve_map_disjoint.
+      - solve_map_disjoint.
+      - instantiate (1 := {| rProp_holds mt ms :=
+                              mt = (mtQ ∪ mtW) ∧
+                              ms = (msQ ∪ msW) |}).
+        simpl. by split.
+    }
+    - simpl. intros vt vs mt' ms'.
+      intros (mtQ' & msQ' & ? & ? & ? & ? & <- & <- & HQ' & [-> ->]).
+      decompose_map_disjoint.
+      exists (mtQ ∪ mtQ'), (msQ ∪ msQ'), mtW, msW.
+      split_and!.
+      + solve_map_disjoint.
+      + solve_map_disjoint.
+      + smap. f_equal. by apply map_union_comm.
+      + smap. f_equal. by apply map_union_comm.
+      + by apply HQ.
       + done.
     - done.
     - done.
@@ -86,16 +109,17 @@ Section SimRules.
     Inv st j i ss Q -∗
     [Pt, Ps, C] st <{j, i}= ss {{ Q }}.
   Proof using Type.
-    unseal.
-    intros ? ? [-> ->]. smap.
-    intros ? ? _ _ [[-> ->] RIH]. smap.
-    intros mt ms _ _ Hinv. smap.
-    unfold sim_lfp. simpl.
-    revert st j i ss Q mt ms Hinv.
+    unfold sim. unseal.
+    intros ? ? [-> ->].
+    intros ? ? _ _ [[-> ->] RIH].
+    intros mt ms _ _ Hinv.
+    intros W mtW msW Hdt Hds HW.
+    smap. unfold sim_def. simpl.
+    revert st j i ss Q mt ms Hinv W mtW msW Hdt Hds HW.
     apply tower.
-    { intros P Hp st j i ss Q mt ms Hinv ? Hq. by apply Hp. }
+    { intros P Hp st j i ss Q mt ms Hinv W mtW msW Hdt Hds HW ? Hq. by apply Hp. }
     clear C.
-    intros C CIH st j i ss Q mt ms Hinv.
+    intros C CIH st j i ss Q mt ms Hinv W mtW msW Hdt Hds HW.
     replace (mt) with (∅ ∪ ∅ ∪ ∅ ∪ mt) by smap.
     replace (ms) with (∅ ∪ ∅ ∪ ∅ ∪ ms) by smap.
     apply RIH; clear RIH.
@@ -106,11 +130,25 @@ Section SimRules.
       intros ? ? _ _ [[-> ->] Hj].
       intros ? ? _ _ [[-> ->] Hi].
       intros mt' ms' _ _ HInv.
+      intros W' mtW' msW' Hdt' Hds' HW'.
       eapply FProgress; [done | done |].
-      apply CIH. by smap.
+      apply CIH; by smap.
     - by smap; apply map_disjoint_empty_r.
     - by smap; apply map_disjoint_empty_r.
     - done.
+    - by smap.
+    - by smap.
+    - done.
+  Qed.
+
+  Lemma sim_frame t s j i Q F:
+    F -∗
+    [Pt, Ps, C] t <{j, i}= s {{ Q }} -∗
+    [Pt, Ps, C] t <{j, i}= s {{ fun vt vs => Q vt vs ∗ F }}.
+  Proof using Type.
+    iIntros "HF Hsim".
+    iApply (sim_mono with "[HF] [//] [//] Hsim").
+    by iIntros (vt vs) "$".
   Qed.
 End SimRules.
 
