theories/RTL/Rules/Hoare.v
@@ -9,7 +9,7 @@ Definition hoare {J I} Pt Ps C Pre ft j i fs Post : rProp :=
   □ (∀ valt vals,
        Pre valt vals -∗
        (* (∀ vt vs, Post vt vs -∗ Ψ vt vs) -∗ *)
-       @sim_lfp rtl_lang rtl_lang J I Pt Ps C
+       @sim rtl_lang rtl_lang J I Pt Ps C
          ([], CallState ft valt) j i ([], CallState fs vals) Post
     )%I.
 
@@ -27,40 +27,27 @@ Section HoareRules.
 
   Context {ft : rtl_function} {j: J} {i: I} {fs : rtl_function}.
 
-  (* Lemma frame F P Q: *)
-  (*   [Pt, Ps, C] {{ P }} ft <{j, i}= fs {{ Q }} -∗ *)
-  (*   [Pt, Ps, C] {{ fun valt vals => P valt vals ∗ F }} ft <{j, i}= fs {{ fun vt vs => Q vt vs ∗ F }}. *)
-  (* Proof using Type. *)
-  (*   unfold hoare. unseal. *)
-  (*   intros ? ? [-> ->] mt ms _ _ [[-> ->] Hsim]. smap. *)
-  (*   split. { by split. } *)
-  (*   intros valt vals. *)
-  (*   intros a b _ _ Hpre. smap. *)
-  (*   destruct Hpre as (mtP & msP & mtF & msF & Ht & Hs & <- & <- & HP & HF). simpl. *)
-  (*   apply Hsim in HP; try apply map_disjoint_empty_r. clear Hsim. *)
-  (*   revert mtP msP mtF msF HF Ht Hs HP. simpl. *)
-  (*   apply tower. *)
-  (*   { admit. } *)
-  (*   clear C. intros C CIH. *)
-  (*   intros mtP msP mtF msF HF Ht Hs Hsim. *)
-  (*   induction Hsim. *)
-  (*   - apply FRelated.  *)
-  (*   simpl. *)
-  (*   iIntros "#H !>" (valt vals Ψ) "[Hpre Hf] Hpost". *)
-  (*   iApply ("H" with "Hpre"). *)
-  (*   iIntros (vt vs) "Hq". iApply "Hpost". *)
-  (*   by iFrame. *)
-  (* Qed. *)
+  Lemma frame F P Q:
+    [Pt, Ps, C] {{ P }} ft <{j, i}= fs {{ Q }} -∗
+    [Pt, Ps, C] {{ fun valt vals => P valt vals ∗ F }} ft <{j, i}= fs {{ fun vt vs => Q vt vs ∗ F }}.
+  Proof using Type.
+    iIntros "#H !>" (valt vals) "[HPre HF]".
+    iIntros (W) "HW".
+    iApply ((sim_mono _ _ _ _ _ _ _ Q) with "[HF] [//] [//] [HPre] HW").
+    - iFrame. iIntros (vt vs) "$".
+    - iApply ("H" with "HPre").
+  Qed.
 
-  (* Lemma consequence P P' Q Q': *)
-  (*   □ (∀ valt vals, P valt vals -∗ P' valt vals) -∗ *)
-  (*   □ (∀ vt vs, Q' vt vs -∗ Q vt vs) -∗ *)
-  (*   [Pt, Ps, C] {{ P' }} ft <{j, i}= fs {{ Q' }} -∗ *)
-  (*   [Pt, Ps, C] {{ P }} ft <{j, i}= fs {{ Q }}. *)
-  (* Proof using Type. *)
-  (*   iIntros "#HP #HQ #H !>" (valt vals Ψ) "Hpre Hpost". *)
-  (*   iApply ("H" with "[Hpre] [Hpost]"). *)
-  (*   - by iApply "HP". *)
-  (*   - iIntros (vt vs) "HQ'". iApply "Hpost". by iApply "HQ". *)
-  (* Qed. *)
+  Lemma consequence P P' Q Q':
+    □ (∀ valt vals, P valt vals -∗ P' valt vals) -∗
+    □ (∀ vt vs, Q' vt vs -∗ Q vt vs) -∗
+    [Pt, Ps, C] {{ P' }} ft <{j, i}= fs {{ Q' }} -∗
+    [Pt, Ps, C] {{ P }} ft <{j, i}= fs {{ Q }}.
+  Proof using Type.
+    iIntros "#HP #HQ #H !>" (valt vals) "Hpre".
+    iIntros (W) "HW".
+    iApply ((sim_mono _ _ _ _ _ _ _ Q') with "[] [//] [//] [Hpre] HW").
+    - by iApply "HQ".
+    - iApply "H". by iApply ("HP" with "Hpre").
+  Qed.
 End HoareRules.
