theories/RTL/Rules/SyncRules.v
@@ -2,6 +2,7 @@ From RSL Require Import Prelude.
 
 From RSL.RTL Require Import RTL Semantics.
 From RSL.Logic Require Import Logic.
+From RSL.Logic Require Import rPropDef.
 
 From RSL.RTL.Rules Require Import CallBind Hoare.
 From RSL.RTL.Rules Require Import TargetRules SourceRules ExploitSourceRules.
@@ -44,6 +45,8 @@ Section SyncRulesDef.
     iIntros (Hpct Hpcs Haddrt Haddrs Hsame Hs) "Hsim Hinj".
     iApply (source_load_exploit with "[Hsim] Hinj"); eauto.
     iIntros (E' lt ls vt vs -> -> ->) "Ht Hs %Hsame' Hinj".
+    iApply (source_load with "[-Hs] Hs"); eauto.
+    iIntros "Hs".
     iApply (target_load with "[-Ht] Ht"); eauto.
     iIntros "Ht".
     iApply "Hsim"; eauto.
@@ -77,7 +80,9 @@ Section SyncRulesDef.
   Proof using Type.
     iIntros (Hpct Hpcs Haddrt Haddrs Hvalt Hvals HsameAddr HsameVal HnE) "Hsim Hinj".
     iApply (source_store_exploit with "[Hsim] Hinj"); eauto.
-    iIntros (E' lt ls vt -> -> ->) "Ht Hs Hinj".
+    iIntros (E' lt ls vt vs -> -> ->) "Ht Hs %Hsame' Hinj".
+    iApply (source_store with "[-Hs] Hs"); eauto.
+    iIntros "Hs".
     iApply (target_store with "[-Ht] Ht"); eauto.
     iIntros "Ht".
     iApply "Hsim"; eauto.
@@ -132,7 +137,9 @@ Section SyncRulesDef.
   Proof using Type.
     iIntros (Hpct Hpcs Hsrct Hsrcs Hrel HnE) "Hsim Hinj".
     iApply (source_free_exploit with "[Hsim] Hinj"); eauto.
-    iIntros (? lt ls vt -> -> ->) "Ht Hs Hinj".
+    iIntros (E' lt ls vt vs -> -> ->) "Ht Hs %Hsame' Hinj".
+    iApply (source_free with "[-Hs] Hs"); eauto.
+    iIntros "Hs".
     iApply (target_free with "[-Ht] Ht"); eauto.
     iIntros "Ht".
     iApply "Hsim".
@@ -155,78 +162,66 @@ Section SyncRulesDef.
     ρs @ regs ⇒ vals ->
     [Pt, Ps, C] {{ Pre }} fnt <{j, i}= fns {{ Post }} -∗
     Pre valt vals -∗
-    □ (∀ j' i' vt vs,
-         ⌜j < j'⌟ -∗
-         ⌜i < i'⌟ -∗
-         Post vt vs -∗
-         [Pt, Ps, C] (ct, State ft pct' (⟦dstt ⇐ vt⟧ρt))
-              <{j', i'}=
-            (cs, State fs pcs' (⟦dsts ⇐ vs⟧ρs)) {{ Q }}) -∗
+    (∀ j' i' vt vs,
+       ⌜j < j'⌟ -∗
+       ⌜i < i'⌟ -∗
+       Post vt vs -∗
+       [Pt, Ps, C] (ct, State ft pct' (⟦dstt ⇐ vt⟧ρt))
+         <{j', i'}=
+       (cs, State fs pcs' (⟦dsts ⇐ vs⟧ρs)) {{ Q }}) -∗
     [Pt, Ps, C] (ct, State ft pct ρt) <{j, i}= (cs, State fs pcs ρs) {{ Q }}.
   Proof using Type.
     intros Hpct Hpcs Hfnt Hfns Hvalt Hvals.
-    iIntros "#Hf Hpre Hsim".
-    iSpecialize ("Hf" with "Hpre").
-    iRevert "Hf Hsim". iStopProof.
-    unseal.
-    intros ? ? [-> ->] mt ms _ _ Hhoare. smap.
-    intros ? ? _ _ [[-> ->] Hsim]. smap.
+    unfold hoare, sim. unseal.
+
+    intros ? ? [-> ->] mtH msH _ _ [[-> ->] Hhoare].
+    intros mtPre msPre ? ? Hpre.
+    intros mtC msC ? ? Hsim.
+    intros W mtW msW Hdt Hds HW. smap.
+
+    decompose_map_disjoint.
+
     eapply chain_source_step with (i' := i). { by econstructor. }
     eapply chain_target_step. { by eexists; econstructor. }
     intros t' Hstept. inv Hstept. simregs. exists j.
+
     eapply fsim_lfp_rtl_call_bind.
     - exists (S j). simpl. lia.
     - exists (S i). simpl. lia.
-    - apply Hhoare.
-    - intros j' i' vt vs mt' ms' Hj Hi H.
-      replace (mt') with (∅ ∪ ∅ ∪ ∅ ∪ mt') by smap.
-      replace (ms') with (∅ ∪ ∅ ∪ ∅ ∪ ms') by smap.
+    - clear Hsim.
+      replace (mtPre ∪ mtC ∪ mtW) with (∅ ∪ mtPre ∪ (mtC ∪ mtW)) by smap.
+      replace (msPre ∪ msC ∪ msW) with (∅ ∪ msPre ∪ (msC ∪ msW)) by smap.
+      apply Hhoare.
+      + solve_map_disjoint.
+      + solve_map_disjoint.
+      + done.
+      + solve_map_disjoint.
+      + solve_map_disjoint.
+      + instantiate (1 := {| rProp_holds mt ms :=
+                             mt = (mtC ∪ mtW) ∧
+                             ms = (msC ∪ msW) |}).
+        by split.
+    - intros j' i' vt vs mt' ms' Hj Hi.
+      intros (mtPost & msPost & ? & ? & ? & ? & <- & <- & Hpost & [-> ->]).
+      decompose_map_disjoint.
+
+      replace (mtPost ∪ (mtC ∪ mtW)) with (mtC ∪ ∅ ∪ ∅ ∪ mtPost ∪ mtW).
+      2:{ smap. f_equal. by apply map_union_comm. }
+      replace (msPost ∪ (msC ∪ msW)) with (msC ∪ ∅ ∪ ∅ ∪ msPost ∪ msW).
+      2:{ smap. f_equal. by apply map_union_comm. }
+
       eapply Hsim.
-      + by smap; apply map_disjoint_empty_r.
-      + by smap; apply map_disjoint_empty_r.
+      + solve_map_disjoint.
+      + solve_map_disjoint.
       + by split.
-      + by smap; apply map_disjoint_empty_r.
-      + by smap; apply map_disjoint_empty_r.
+      + solve_map_disjoint.
+      + solve_map_disjoint.
       + by split.
-      + by smap; apply map_disjoint_empty_r.
-      + by smap; apply map_disjoint_empty_r.
+      + solve_map_disjoint.
+      + solve_map_disjoint.
       + assumption.
+      + solve_map_disjoint.
+      + solve_map_disjoint.
+      + done.
   Qed.
-
-  (* Lemma both_call_framed Pre Post F ct ft pct ρt j i cs fs pcs ρs Q *)
-  (*   pct' pcs' dstt dsts fnamet fnames regt regs valt vals fnt fns: *)
-  (*   ft@pct is <<{ dstt := @call fnamet regt -> pct' }>> -> *)
-  (*   fs@pcs is <<{ dsts := @call fnames regs -> pcs' }>> -> *)
-  (*   find_fun Pt fnamet = Some fnt -> *)
-  (*   find_fun Ps fnames = Some fns -> *)
-  (*   ρt @ regt ⇒ valt -> *)
-  (*   ρs @ regs ⇒ vals -> *)
-  (*   [Pt, Ps, C] {{ Pre }} fnt <{j, i}= fns {{ Post }} -∗ *)
-  (*   Pre valt vals -∗ *)
-  (*   F -∗ *)
-  (*   □ (∀ j' i' vt vs, *)
-  (*        ⌜j < j'⌟ -∗ *)
-  (*        ⌜i < i'⌟ -∗ *)
-  (*        Post vt vs -∗ *)
-  (*        F -∗ *)
-  (*        [Pt, Ps, C] (ct, State ft pct' (⟦dstt ⇐ vt⟧ρt)) *)
-  (*             <{j', i'}= *)
-  (*           (cs, State fs pcs' (⟦dsts ⇐ vs⟧ρs)) {{ Q }}) -∗ *)
-  (*   [Pt, Ps, C] (ct, State ft pct ρt) <{j, i}= (cs, State fs pcs ρs) {{ Q }}. *)
-  (* Proof using Type. *)
-  (*   intros Hpct Hpcs Hfnt Hfns Hvalt Hvals. *)
-  (*   iIntros "Hhoare Hpre HF #Hsim". *)
-  (*   iApply (both_call with "[Hhoare] [Hpre HF]"). *)
-  (*   - done. *)
-  (*   - done. *)
-  (*   - done. *)
-  (*   - done. *)
-  (*   - done. *)
-  (*   - done. *)
-  (*   - iApply (frame with "Hhoare"). *)
-  (*   - iFrame. iApply "HF". *)
-  (*   - iModIntro. iIntros (j' i' vt vs Hj Hi) "[HPost HP2]". *)
-  (*     iApply ("Hsim" $! j' i' vt vs Hj Hi with "HPost HP2"). *)
-  (* Qed. *)
-
 End SyncRulesDef.
